\documentclass[12pt]{article}
\usepackage{amsmath}


\begin{document}


3.1

Find the OGFs for each of the following sequences:

\begin{equation}
\{ 2^{k+1}\}_{k \geq 0}, \{k2^{k+1} \}_{k \geq 0}, \{kH_{k}\}_{k \geq 1}, \{k^3\}_{k \geq 2}. \nonumber
\end{equation}


1)

\begin{equation}
A_{1}(z) = \sum_{k \geq 0}2^{k+1}z^k = 2\sum_{k \geq 0}2^kz^k = \frac{2}{1-2z} \nonumber
\end{equation}

2)

\begin{equation}
A_{2}(z) = \sum_{k \geq 0}k2^{k+1}z^k  = \sum_{k \geq 0}(k+1)2^{k+1}z^k - \sum_{k \geq 0}2^{k+1}z^k \nonumber
\end{equation}

\begin{equation}
A_{2.1}(z) = \sum_{k \geq 0}(k + 1)2^{k+1}z^k \nonumber
\end{equation}

\begin{equation}
\int_0^z A_{2.1}(t) = \sum_{k \geq 1}\frac{k2^k}{k}z^k = \sum_{k \geq 1} 2^kz^k = \frac{1}{1-2z} - 1\nonumber
\end{equation}

\begin{equation}
A_{2.1}(z) = \frac{2}{(1-2z)^2} \nonumber
\end{equation}

\begin{equation}
A_{2}(z) = \frac{4z}{(1 - 2z)^2} \nonumber
\end{equation}

3)

\begin{equation}
A_{3}(z) = \sum_{k \geq 1} kH_kz^k =  \dots \nonumber
\end{equation}

4)

\begin{equation}
A_{4}(z) = \sum_{k \geq 2}{k^3z^k} = \dots \nonumber
\end{equation}

3.2

Find ${[z^N]}$ for each of the following OGFs:

\begin{equation}
\frac{1}{(1 - 3z)^4}, (1 - z)^2ln\frac{1}{1 - z}, \frac{1}{(1 - 2z^2)^2} \nonumber
\end{equation}

1)

\begin{equation}
    \frac{1}{(1-3z)^2} = \sum_{N \geq 0}3^Nz^N \sum_{N \geq 0}3^Nz^N = \sum_{N \geq 0} \bigg( \sum_{0 \leq k \leq N}3^k3^{N-k} \bigg) z^N = \sum_{N \geq 0}N3^NZ^N \nonumber
\end{equation}

\begin{equation}
\begin{split}
    \bigg(\sum_{N \geq 0}N3^Nz^N\bigg)\bigg(\sum_{N \geq 0}N3^Nz^N\bigg) = \sum_{N \geq 0} \bigg( \sum_{0 \leq k \ leq N}k3^k(N-k)3^{N-k} \bigg)z^N =\\
    \sum_{N \geq 0} \bigg( \sum_{0 \leq k \leq N}k(N - k) \bigg)3^Nz^N = \sum_{N \geq 0} \frac{1}{6}(N-1)N(N+1)3^Nz^N \nonumber
\end{split}
\end{equation}

3.4

Prove that

\begin{equation}
\sum_{1 \leq k \leq N} H_k = (N + 1)(H_{N + 1} - 1) \nonumber
\end{equation}

\begin{equation}
\begin{split}
\sum_{1 \leq k \leq N} H_k & = \underbrace{1 + \dots + 1}_{N} + \underbrace{\frac{1}{2} + \dots + \frac{1}{2}}_{N - 1} + \dots + \underbrace{\frac{1}{N-1} + \frac{1}{N-1}} + \frac{1}{N} \\
                           & = \sum_{1 \leq i \leq N}\frac{1}{i}(N - i + 1) = \sum_{1 \leq i \leq N}\frac{N+1}{i} - \sum{1 \leq i \leq N}1\\
                           & = (N + 1)H_N - N = (N + 1)H_N - \frac{(N + 1)N}{N + 1} = (N + 1)(H_N - \frac{N+1}{N+1} + \frac{1}{N+1})\\
                           & = (N + 1)(H_{N+1} - 1)\nonumber
\end{split}
\end{equation}


3.6

Find the OGF for

\begin{equation}
\left\{\sum_{0 < k < n} \frac{1}{k(n - k)}\right\}_{n > 1} \nonumber
\end{equation}

\begin{equation}
    \sum_{0 < k < n}\frac{1}{k(n-k)} = \sum_{0 < k < n}\frac{1}{n} \bigg( \frac{1}{k} + \frac{1}{n - k} \bigg)\\
    = \sum_{0 < k < n} \bigg( \frac{1}{nk} + \frac{1}{n(n-k)} \bigg)\\
    = \sum_{0 < k < n} \frac{2}{nk} = \frac{2}{n}H_{n-1} \nonumber
\end{equation}

\begin{equation}
A(z) = \sum_{n > 1}\frac{2}{n}H_{n - 1}z^n \nonumber
\end{equation}

\begin{equation}
    A'(z) = \sum_{n > 1}(n + 1) \frac{2H_n}{n + 1} z^n = 2\sum_{n > 1} H_nz^n = \frac{2}{1 - z}ln\frac{1}{1 - z} \nonumber
\end{equation}

\begin{equation}
    A(z) = ln^2\bigg(\frac{1}{1 - z}\bigg) + C \nonumber
\end{equation}

3.7

Find the OGF for ${ \left\{H_k/k \right\}_{k \geq 1} }$

\begin{equation}
A(z) = \sum_{n \geq 1}\frac{H_n}{n}z^n\nonumber
\end{equation}


\begin{equation}
A'(z) = \sum_{n \geq 1}(n + 1)\frac{H_{n+1}}{n + 1}z^{n + 1} = \\
\sum_{n \geq 1} H_{n + 1}z_{n+1} = \\
\sum_{n \geq 2} H_{n}z^{n} = \frac{1}{1-z}ln\frac{1}{1-z} - 1 \nonumber
\end{equation}

\begin{equation}
A(z) = \frac{1}{2}ln^2\bigg(\frac{1}{1-z} \bigg) - z + C \nonumber
\end{equation}

3.9

Find the EGFs for each of the following seqences:

\begin{equation}
\left\{ 2^{k+1}\right\}_{k \geq 0}, \left\{k2^{k+1}\right\}_{k \geq 0}, \\
\left\{k^3\right\}_{k \geq 2} \nonumber
\end{equation}

\begin{equation}
A_1(z) = \sum_{k \geq 0}2^{k+1}\frac{z^k}{k!} = \\
2\sum_{k \geq 0}2^k\frac{z^k}{k!} = 2e^{2z}\nonumber
\end{equation}

\begin{equation}
A_2(z) = \sum_{k \geq 0}k2^{k+1}\frac{z^k}{k!} \nonumber
\end{equation}

\begin{equation}
\frac{A_2(z) - A_2(0)}{z} = \frac{A_2(z)}{z} = \\
\sum_{k \geq 1}\frac{(k+1)2^{k+2}}{(k+1)}\frac{z^k}{k!} = \\
\sum_{k \geq 1}2^{k+2}\frac{z^k}{k!} = \\
4\sum_{k \geq 1}2^k\frac{z^k}{k!} = 4e^{2z}\nonumber
\end{equation}

\begin{equation}
A_2(z) = 4ze^{2z} \nonumber
\end{equation}

\begin{equation}
A_3(z) = \sum_{k \geq 2} k^3 \frac{z^k}{k!} \nonumber
\end{equation}

\begin{equation}
\frac{A_3(z) - A_3(0)}{z} = \frac{A_3(z)}{z} = \\
\sum_{k \geq 2} \frac{(k+1)^3}{(k+1)} \frac{z^k}{k!} = B(z) \nonumber
\end{equation}

\begin{equation}
\frac{B(z) - B(0)}{z} = \sum_{k \geq 2}\frac{(k+2)^2}{(k+2)}\frac{z^k}{k!} =\\
\sum_{k \geq 2}(k + 2)\frac{z^k}{k!} = ze^z + 2e^z \nonumber
\end{equation}

\begin{equation}
A_3(z) = z^2e^z(z + 2) \nonumber
\end{equation}

3.16

Use generating functions to solve the following recurrences:

\begin{equation}
\begin{aligned}
& a_n = -a_{n - 1} + 6a_{n - 2} \qquad \text{ for ${n > 1}$ with ${a_0 = 0}$ and ${a_1 = 1}$;} \\
& a_n = 11a_{n - 2} + 6a_{n - 3} \qquad \text{ for ${n > 2}$ with ${a_0 = 0}$ and ${a_1 = a_2 = 1}$;} \\
& a_n = 3a_{n - 1} - 4a_{n - 2} \qquad \text{ for ${n > 1}$ with ${a_0 = 0}$ and ${a_1 = 1}$;} \\
& a_n = a_{n - 1} - a_{n - 2} \qquad \text{ for ${n > 1}$ with ${a_0 = 0}$ and ${a_1 = 1}$} \nonumber
\end{aligned}
\end{equation}

1)

\begin{equation}
\begin{aligned}
a_nz^n & = -a_{n - 1}z^n + 6a_{n - 2}z^n + \delta_1z^n \\
\sum_{n \geq 0} a_nz^n & = -\sum_{n \geq 0}a_{n-1}z^n + 6\sum_{n \geq 0}a_{n - 2}z^n + \sum_{n \geq 0}z\\
\sum_{n \geq 0} a_nz^n & = -z \sum_{n \geq 0}a_{n-1}z^{n-1} + 6z^2\sum_{n \geq 0}a_{n-2}z^{n-2} + \sum_{n \geq 0}z \\
a(z) & = -za(z) + 6z^2a(z) + z \\
a(z) & = \frac{z}{1 + z - 6z^2} = \frac{z}{(1 - (-3)z)(1 - 2z)} \\
a(z) & = \frac{1}{5}\left(\frac{1}{1 - 2z} - \frac{1}{1 - (-3)z} \right) \\
a_n & = \frac{1}{5}\left(({2^n} - (-3)^n\right) \nonumber
\end{aligned}
\end{equation}

2)

\begin{equation}
\begin{aligned}
a_n & = 11a_{n - 2} + 6a_{n - 3} + \delta_1 + \delta_2 \\
\sum_{n \geq 0} a_nz^n & = 11z^2\sum_{n \geq 0}a_{n - 2}z^{n - 2} + 6z^3\sum_{n \geq 0} a_{n - 3}z^{n - 3} + z + z^2 \\
a(z) & = 11z^2a(z) + 6z^3a(z) + z + z^2 \\
a(z) & = \frac{z + z^2}{1 - 11z^2 - 6z^3} \\
\nonumber
\end{aligned}
\end{equation}

3)

\begin{equation}
\begin{aligned}
a_n & = 3a_{n - 1} - 4a_{n - 2} \qquad \text{for ${n > 1}$ with ${a_0 = 0}$ and ${a_1 = 1}$} \\
g(z) & = 1 - 3z + 4z^2 \\
f(z) & = z \\
a(z) & = \frac{z}{1 - 3z + 4z^2} \\
\nonumber
\end{aligned}
\end{equation}

3.17

Solve the recurrence:

\begin{equation}
a_n = 5a_{n - 1} - 8a_{n - 2} + 4a_{n - 3} \qquad
\text{for ${n > 2}$ with ${a_0 = 1, a_1 = 2, a_2 = 4.}$} \nonumber
\end{equation}

\begin{equation}
\begin{split}
    a_n & = 5a_{n - 1} - 8a_{n - 2} + 4a_{n - 3} + \delta_{n1} - \delta_{n2} \\
    g(z) & = 1 - 5z + 8z^2 - 4z^3 = (1 - z)(1 - 2z)^2 \\
    f(z) & = z - z^2 \\
    a(z) & = \frac{z(1 - z)}{(1 - z)(1 - 2z)^2} = \frac{z}{(1 - 2z)^2} \\
    a_n & = n2^{n - 1} \nonumber
\end{split}
\end{equation}

\end{document}
