\documentclass[12pt]{article}
\usepackage{amsmath}

\begin{document}

2.11

Solve the reccurence:

\begin{equation}
na_{n} = (n - 2)a_{n - 1} + 2  \qquad \text{for ${n > 1}$ with ${a_{1} = 1}$}. \nonumber
\end{equation}

Solution. Use the summation factor ${n - 1}$:

\begin{equation}
\begin{split}
n(n - 1)a_{n}   & = (n - 1)(n - 2)a_{n - 1} + 2(n - 1) \\
		& = (n - 2)(n - 3)a_{n-2} + 2(n - 2) + 2(n - 1) \\
		& = 2(1 + 2 + \dots + n - 1) \\
		& = n(n-1) \\
          a_{n} & = 1 \qquad \text{for ${n \geq 1}$}\nonumber
\end{split}
\end{equation}

Easier solution. Compute ${a_{2} = 1}$, think for a moment, and then prove
by induction that ${a_{n} = 1}$ for all ${n \geq 1}$.

\bigskip
2.12.

Solve the reccurence

\begin{equation}
a_{n} = 2a_{n-1} + 1 \qquad \text{for ${n > 1}$ with ${a_{1} = 1}$.} \nonumber
\end{equation}

\begin{equation}
\frac{a_{n}}{2^n} = \frac{a_{n-1}}{2^{n-1}} + \frac{1}{2^n} \nonumber
\end{equation}

\begin{equation}
\begin{split}
\frac{a_{n}}{2^n} & = \frac{1}{2^n} + \frac{1}{2^{n-1}} + \dots + \frac{1}{2} + 1 \\
                  & = \sum_{0 \leq i \leq n}\frac{1}{2^i} = \frac{2^{n+1} - 1}{2^n}\nonumber
\end{split}
\end{equation}


\begin{equation}
a^n = 2^n - 1 \nonumber
\end{equation}

\bigskip

2.13

Solve the reccurence

\begin{equation}
a_{n} = \frac{n}{n + 1}a_{n-1} + 1 \qquad \text{for ${n > 0}$ with ${a_{0} = 1}$} \nonumber
\end{equation}

\begin{equation}
\begin{split}
(n + 1)a_{n} & = 1 + n + na_{n - 1} \\
	     & = 1 + n + 1 + (n - 1) + na_{n - 2} \\
	     & = 1 + n + n + (n - 1) + \dots + 1 \\
	     & = \frac{(n + 1)(n + 2)}{2} \nonumber
\end{split}
\end{equation}

\begin{equation}
	a_{n} = (n + 2)/2 \nonumber
\end{equation}


\bigskip

2.15
Solve the reccurence

\begin{equation}
na_{n} = (n + 1)a_{n - 1} + 2n \qquad \text{for ${n > 0}$ with ${a_{0} = 0}$.} \nonumber
\end{equation}

\begin{equation}
\begin{split}
\frac{a_{n}}{n + 1} & = \frac{a_{n - 1}}{n} + \frac{2}{n + 1} = \frac{a_{n - 2}}{n - 1} + \frac{2}{n} + \frac{2}{n + 1} \\
	= 2(\sum_{1 \leq i \leq n + 1}\frac{1}{i} - 1) = 2(H_{n + 1} - 1) \nonumber
\end{split}
\end{equation}


\begin{equation}
a_{n} = 2(n + 1)(H_{n + 1} - 1) \nonumber
\end{equation}

\end{document}
