\documentclass[12pt]{article}
\usepackage{amsmath}
\usepackage{graphicx}

\begin{document}

4.2

Show that

\begin{equation}
\frac{N}{N + 1} = 1 + \mathcal{O}\left(\frac{1}{N}\right) \qquad \text{and}
\qquad \frac{N}{N + 1} \sim 1 - \frac{1}{N}. \nonumber
\end{equation}

\begin{equation}
\frac{N}{N + 1} = 1 - \frac{1}{N + 1} \nonumber
\end{equation}

\begin{equation}
\left|- \frac{1}{N + 1} \frac{N}{1} \right| < 1 \Rightarrow -\frac{1}{N + 1} =
\mathcal{O}\left(\frac{1}{N}\right) \Rightarrow \frac{N}{N + 1} =
1 + \mathcal{O}\left(\frac{1}{N}\right)\nonumber
\end{equation}

\begin{equation}
\begin{split}
\left(-\frac{1}{N + 1}\right)\left(-\frac{N}{1}\right) = \frac{N}{N + 1} =
1 - \frac{1}{N + 1} \rightarrow 1 \text{ as } N \rightarrow \infty \Rightarrow\\
\frac{N}{N + 1} \sim 1 - \frac{1}{N}
\nonumber
\end{split}
\end{equation}

4.14

Use theorem 4.1 to find an asymptotic solution to the recurrence:

\[
a_n = 5a_{n - 1} - 8a_{n - 2} + 4a_{n - 3} \qquad \text{for $n > 2$ with
    $a_0 = 1$, $a_1 = 2$ and $a_2 = 4$} \nonumber
\]

\[
\begin{split}
g(z) & = 1 - 5z + 8z^2 - 4z^3 = (z - 1)(-4z^2 + 4z - 1) = (1 - z)(1 - 2z)^2 \\
f(z) & = (1 + 2z + 4z^2)(1 - 5z + 8z^2 - 4z^3)(mod\ z^3) \\
     & = (1 - 5z + 8z^2 + 2z - 10z^2 + 4z^2) = (1 - 3z + 2z^2)
     = 2(z - \frac{1}{2})(z - 1) \\
     & = (2z - 1)(z - 1) \\
a(z) & = \frac{1}{1 - 2z} \\
C & = 1\frac{(-2)^21}{16 - 24/2} = \frac{4}{4} = 1 \\
[z^n]\frac{f(z)}{g(z)} & \sim 2^nn
\end{split}
\]

4.15

Use theorem 4.1 to find an asymptotic solution to the reccurence:

\[
a_n = 2a_{n - 2} - a_{n - 4} \qquad \text{for $n > 4$ with $a_0 = a_1 = 0$
    and $a_2 = a_3 = 1$}
\]

\[
\begin{split}
g(z) & = 1 - 2z^2 + z^4 = (1 - z^2)^2 \\
f(z) & = (1 - 2z^2 + z^4)(z^2 + z^3)(mod z^4) = (z^2) \\
a(z) & = \frac{(z^2)}{(1 - z^2)^2}\\
& \text{Here $\beta = 1$, $\nu = 2, g''(1) = 8$ and $f(1) = 1$ so Theorem 4.1 tells that} \\
a_n & \sim \frac{1}{4}n
\end{split}
\]

4.16

Use theorem 4.1 to find an asymptotic solution to the recurrence:

\[
a_n = 3a_{n - 1} - 3a_{n - 2} + a_{n - 3} \qquad
\text{for $n > 2$ with $a_0 = a_1 = 0$ and $a_2 = 1$.}
\]

\[
\begin{split}
g(z) & = 1 - 3z + 3z^2 - z^3 = (z - 1)(-z^2 + 2z - 1) = (1 - z)^3 \\
f(z) & = (1 - 3z - 3z^2 - z^3)(z^2)(\text{mod}\ z^3) = (z^2) \\
a(z) & = \frac{z^2}{(1 - z)^3} \\
& \text{Here $\beta = 1$, $\nu = 3$, $g^{(3)}(1) = -6$
    and $f(1) = 1$}\\
a_n & \sim 3\frac{(-1)^3}{-6}n^2 = \frac{1}{2}n^2
\end{split}
\]

4.21

Expand $ln(1 - x + x^2)$ as $x \rightarrow 0$, to within $\mathcal{O}(x^4)$.

Substitute $(x^2 - x)$ with $y$. $y \rightarrow 0$ as $x \rightarrow 0$.

\[
\begin{split}
ln(1 + y) & = y - \frac{y^2}{2} + \frac{y^3}{3} + \mathcal{O}(y^4) \\
ln(1 + x^2 - x) & = x^2 - x - \frac{(x^2 - x)^2}{2} + \frac{(x^2 - x)^3}{3} +
    \mathcal{O}((x^2 - x)^4) \\
    & = -x + x^2 - \frac{x^4}{2} + x^3 - \frac{x^2}{2} + \frac{(x^2 - x)^3}{3} +
    \mathcal{O}(x^4) \\
    & = -x + \frac{x^2}{2} + x^3 - \frac{x^3}{3} + \mathcal{O}(x^4) \\
    & = -x + \frac{x^2}{2} + \frac{2x^3}{3} + \mathcal{O}(x^4)
\end{split}
\]

4.23

Give an asymptotic expansion for $\frac{N}{N - 1}ln\frac{N}{N - 1}$.

\[
\begin{split}
\frac{N}{N - 1}ln\frac{N}{N - 1} & = \left(1 + \frac{1}{N - 1}\right)ln\frac{N}{N - 1}
    = \left(1 + \frac{1}{N - 1}\right)ln\left(1 + \frac{1}{N - 1}\right) \\
& \sim \frac{1}{N - 1} - \frac{1}{2(N - 1)^2} +
    \mathcal{O}\left(\frac{1}{(N - 1)^3}\right)
\end{split}
\]

\end{document}
